experiments/Tests.v
@@ -1,0 +1,38 @@
+Require Import Lam2Gmu.
+Require Import TLC.LibLN.
+
+Notation "@ n" := (typ_bvar n) (at level 42).
+Notation "# n" := (trm_bvar n) (at level 42).
+
+Definition id := trm_tabs (trm_abs (@0) (#0)).
+Definition id_typ := typ_all (typ_arrow (@0) (@0)).
+
+Hint Constructors type term wft.
+
+Lemma well_formed_id :
+  term id
+  /\ type id_typ
+  /\ wft empty empty id_typ.
+  intuition.
+  (* TODO create tactics to automate such simple proofs *)
+  - econstructor. intros.
+    econstructor; cbn; case_if. econstructor.
+    intros.
+    econstructor.
+  - econstructor.
+    intros.
+    repeat (econstructor; case_if).
+  - econstructor.
+    intros.
+    econstructor; case_if; econstructor.
+    + eauto.
+    + eauto.
+      (* TODO FIXME:
+All the remaining goals are on the shelf.
+subgoal 1 (ID 794) is:
+ fset var
+Error: Attempt to save a proof with shelved goals (in proof well_formed_id)
+      *)
+Admitted.
+
+(* Lemma well_typed_id : empty empty ⊢ id :~ id_typ. *)
